



$$m\ddot{x} = -Kx$$

$$\ddot{x} = -\frac{K}{m}x$$

$$\frac{K}{m} = 1 \text{ s}^{-2}$$

$$\underline{X}(t) = \begin{pmatrix} x(t) \\ v(t) \end{pmatrix}$$

$$\dot{\underline{X}}(t) = \begin{pmatrix} \dot{x}(t) \\ \dot{v}(t) \end{pmatrix} = \begin{pmatrix} v(t) \\ -\frac{K}{m}x(t) \end{pmatrix}$$

$$\underline{X}(0) = \begin{pmatrix} 1 \text{ m} \\ 0 \text{ m/s} \end{pmatrix}$$

$$h = 0,1 \text{ s}$$

Metodo di Eulero:

$$\underline{X}(0+h) = \underline{X}(0) + h \dot{\underline{X}}(0) =$$

$$= \begin{pmatrix} 1 \text{ m} \\ 0 \text{ m/s} \end{pmatrix} + 0,1 \text{ s} \begin{pmatrix} v(0) \\ -\frac{K}{m}x(0) \end{pmatrix} =$$

$$= \begin{pmatrix} 1 \text{ m} \\ 0 \text{ m/s} \end{pmatrix} + 0,1 \text{ s} \begin{pmatrix} 0 \text{ m/s} \\ -1 \text{ s}^{-2} \cdot 1 \text{ m} \end{pmatrix} =$$

$$= \begin{pmatrix} 1 \text{ m} + 0,1 \text{ s} \cdot 0 \text{ m/s} \\ 0 \text{ m/s} + 0,1 \text{ s} \cdot (-1 \text{ s}^{-2} \cdot 1 \text{ m}) \end{pmatrix} = \begin{pmatrix} 1 \text{ m} \\ -0,1 \text{ m/s} \end{pmatrix}$$